feat: defs and lemmas for lf_path and shorter_ss.

common.v
@@ -1,5 +1,7 @@
-Require Import Coq.Logic.Classical_Prop.
 Require Export ZArith.
+Require Export logic.
+Require Import Fourier.
+(*Require Import FunctionalExtensionality.*)
 (*Require Export SMTC.Tactic.
 Require Import SMTC.Integers.*)
 
@@ -12,7 +14,8 @@ Set Implicit Arguments.
 
 (**)
 
-Definition state : Type := nat -> Z.
+(*Definition state : Type := nat -> Z.*)
+Definition state : Type := Z.
 Definition sseq : Type := nat -> state.
 
 Definition nth (n : nat) (ss : sseq) : state :=
@@ -32,15 +35,6 @@ Proof.
   rewrite plus_comm.
   reflexivity.
 Qed.
-
-(*Lemma skipn_nth: forall A:Type, forall l:list A, forall n m:nat, forall d:A,
-  nth m (skipn n l) d = nth (n+m) l d.
-Proof.
-  intros A l.
-  induction l; intros; 
-    destruct m; destruct n; simpl; auto.
-Qed.
-*)
 
 Lemma state_sseq :
   forall (s:state), (fun _ => s).[0] = s.
@@ -66,7 +60,6 @@ Definition prop : Type := state -> Prop.
 Fixpoint path (T : trans) (ss : sseq) (o len : nat) : Prop :=
   match len with
   | O => True
-  (*| S O => T ss.[o] ss.[o+1]*)
   | S len' => path T ss o len' /\ T ss.[o+len'] ss.[o+len]
   end.
 
@@ -76,38 +69,37 @@ Fixpoint invariance (P : prop) (ss : sseq) (len : nat) : Prop :=
   | S len' => invariance P ss len' /\ P ss.[len]
   end.
 
+(*
 Fixpoint neq_states (si sj : state) (size : nat) : Prop :=
   match size with
   | O => True
-  (*| S O => ~ (si 0 = sj 0)*)
   | S sz' => neq_states si sj sz' \/ ~ (si sz' = sj sz')
   end.
+*)
 
-Fixpoint no_loop' (ss : sseq) (size o m n: nat) : Prop :=
+Fixpoint no_loop' (ss : sseq) (o m n: nat) : Prop :=
   match n with
-  | O => neq_states (ss.[o+m]) (ss.[o+n]) size
-  | S n' => no_loop' ss size o m n' /\ 
-      neq_states (ss.[o+m]) (ss.[o+n]) size
+  | O => ss.[o+m] <> ss.[o]
+  | S n' => no_loop' ss o m n' /\ ss.[o+m] <> ss.[o+n]
   end.
 
-Fixpoint no_loop (ss : sseq) (size o k : nat) : Prop :=
+Fixpoint no_loop (ss : sseq) (o k : nat) : Prop :=
   match k with
   | O => True
-  (*| 1 => no_loop' ss size o 1 0*)
-  | S k' => no_loop' ss size o k k' /\ no_loop ss size o k'
+  | S k' => no_loop' ss o k k' /\ no_loop ss o k'
   end.
 
-Definition loop_free (T : trans) (ss : sseq) (size o k: nat) : Prop :=
-  path T ss o k /\ no_loop ss size o k.
+Definition loop_free (T : trans) (ss : sseq) (o k: nat) : Prop :=
+  path T ss o k /\ no_loop ss o k.
 
-Definition lasso (I : init) (T : trans) (P : prop) (size k : nat) : Prop :=
+Definition lasso (I : init) (T : trans) (P : prop) (k : nat) : Prop :=
   forall ss : sseq,
-  ~ (I ss.[0] /\ loop_free T ss size 0 k).
+  ~ (I ss.[0] /\ loop_free T ss 0 k).
 
 Definition violate_loop_free (I : init) (T : trans)
-           (P : prop) (size k: nat) : Prop :=
+           (P : prop) (k: nat) : Prop :=
   forall ss : sseq,
-  ~ (loop_free T ss size 0 k /\ ~ P ss.[k ]).
+  ~ (loop_free T ss 0 k /\ ~ P ss.[k ]).
 
 
 Definition prop_k_init (I : init) (T : trans) (P : prop) (k : nat) : Prop :=
@@ -120,9 +112,9 @@ Fixpoint safety_k (I : init) (T : trans) (P : prop) (k : nat) : Prop :=
   | S k' => safety_k I T P k' /\ prop_k_init I T P k
   end.
 
-Definition prop_k_init_lf  (I : init) (T : trans) (P : prop) (size k : nat) : Prop :=
+Definition prop_k_init_lf  (I : init) (T : trans) (P : prop) (k : nat) : Prop :=
   forall ss : sseq,
-  ~ (I ss.[0] /\ loop_free T ss size 0 k /\ ~ P ss.[k]).
+  ~ (I ss.[0] /\ loop_free T ss 0 k /\ ~ P ss.[k]).
 
 Fixpoint safety_k_offset (P : prop) (ss : sseq) (o k: nat) : Prop :=
   match k with
@@ -132,87 +124,27 @@ Fixpoint safety_k_offset (P : prop) (ss : sseq) (o k: nat) : Prop :=
 
 (**)
 
-Lemma not_and_imply3 :
-  forall (p1 p2 p3:Prop), 
-  ~(p1 /\ p2 /\ ~p3) -> (p1 /\ p2 -> p3).
-Proof.
-  intros. tauto.
-  (*revert H0.
-  apply or_to_imply.
-  apply not_and_or in H.
-  destruct H.
-  - left. apply or_not_and. auto.
-  - apply not_and_or in H.
-    destruct H.
-    + left. apply or_not_and. auto.
-    + right. apply NNPP in H. apply H.*)
-Qed.
-
-Lemma imply_to_not_and3 :
-  forall (p1 p2 p3:Prop), 
-  (p1 /\ p2 -> p3) -> ~(p1 /\ p2 /\ ~p3).
-Proof.
-  intros. tauto.
-  (*apply or_not_and.
-  apply imply_to_or in H.
-  destruct H. 
-  - apply not_and_or in H.
-    destruct H. 
-    + left. apply H.
-    + right. apply or_not_and. auto.
-  - right. apply or_not_and. auto.*)
-Qed.
-
-Lemma and_to_imply_premise :
-  forall (p1 p2 p3:Prop),
-  (p1 /\ p2 -> p3) -> (p1 -> p2 -> p3).
-Proof.
-  intros. tauto.
-  (*apply imply_to_or in H.
-  destruct H.
-  - apply not_and_or in H.
-    firstorder.
-  - apply H.*)
-Qed.
-
-Lemma not_ntq_not_pq :
-  forall (p q:Prop),
-    ~(p /\ True /\ q) -> ~(p /\ q).
-Proof.
-  firstorder.
-Qed.
-
 Lemma safety_path_lf :
-  forall (I:init) (T:trans) (P:prop) (size:nat),
+  forall (I:init) (T:trans) (P:prop),
   forall (i:nat),
     prop_k_init I T P i ->
-    (forall (size:nat), prop_k_init_lf I T P size i).
+    prop_k_init_lf I T P i.
 Proof.
   intros.
   unfold prop_k_init in H.
   unfold prop_k_init_lf.
   unfold loop_free.
   intros.
-
   assert (forall (p1 p2 p3 p4:Prop), (p1 /\ p2 /\ p3 -> p4) -> (~(p1 /\ (p2 /\ p3) /\ ~p4))) by firstorder.
-
-  apply H0.
+  apply H0; clear H0.
   intros.
-  decompose [and] H1.
-  revert H4; revert H2.
-
-  apply and_to_imply_premise.
+  decompose [and] H0; clear H0.
+  revert H3; revert H1.
+  apply and_imply_premise.
   apply or_to_imply.
-
-  assert (forall (p q:Prop), ~(p /\ ~q) -> (~p \/ q)).
-  intros.
-  apply not_and_or in H2.
-  destruct H2.
-  left; apply H2. right; apply NNPP; apply H2.
-
-  apply H2. 
+  apply not_and_or'. 
   assert (forall (p1 p2 p3:Prop), ~(p1 /\ p2 /\ p3) -> ~((p1 /\ p2) /\ p3)) by firstorder.
-  apply H3.
+  apply H0; clear H0.
   apply H.
 Qed.
 
@@ -244,32 +176,29 @@ Proof.
     + clear IHi.
       rewrite skipn_nth.
       rewrite skipn_nth.
-      (*replace (j + i) with (i + j).*)
-      (*replace (j + S i) with (S i + j).*)
       simpl in *.
       decompose [and] H. clear H.
       destruct i.
       * simpl in *.
-        (*rewrite Nat.add_1_r in H.
-        rewrite Nat.add_0_r in H.*)
         auto.
-      * (*rewrite Nat.add_1_r in H.*)
-        auto.
+      * auto.
 Qed.
 
-Lemma skipn_no_loop' : forall (size i j k : nat),
+Lemma skipn_no_loop' : forall (i j k : nat),
   forall ss : sseq,
-  no_loop' ss size j k i ->
-  no_loop' (skipn j ss) size 0 k i.
+  no_loop' ss j k i ->
+  no_loop' (skipn j ss) 0 k i.
 Proof.
   intros.
   destruct i.
   - simpl in *.
     do 2 rewrite skipn_nth.
+    rewrite -> Nat.add_0_r.
     apply H.
   - induction i.
     + simpl in *.
       do 3 rewrite skipn_nth.
+      rewrite -> Nat.add_0_r.
       apply H.
     + simpl.
       split.
@@ -280,21 +209,21 @@ Proof.
         tauto.
 Qed.
 
-Lemma skipn_no_loop : forall (size i j : nat),
+Lemma skipn_no_loop : forall (i j : nat),
   forall ss : sseq,
-  no_loop ss size j i -> no_loop (skipn j ss) size 0 i.
+  no_loop ss j i -> no_loop (skipn j ss) 0 i.
 Proof.
   intros.
   induction i.
   - auto.
 
-  - assert (H1 : no_loop ss size j i /\ no_loop' ss size j (S i) i)
+  - assert (H1 : no_loop ss j i /\ no_loop' ss j (S i) i)
       by ( destruct i; firstorder; rewrite <- plus_n_O in *).
     clear H.
 
-    assert ( H :no_loop (skipn j ss) size 0 i /\
-      no_loop' (skipn j ss) size 0 (S i) i -> 
-      no_loop (skipn j ss) size 0 (S i) ).
+    assert ( H :no_loop (skipn j ss) 0 i /\
+      no_loop' (skipn j ss) 0 (S i) i -> 
+      no_loop (skipn j ss) 0 (S i) ).
     intros.
     destruct i; firstorder; rewrite <- plus_n_O in *.
     apply H.
@@ -345,38 +274,53 @@ Qed.
 
 (**)
 
-Lemma split_no_loop_former : forall (ss : sseq) (size j i : nat),
-  no_loop ss size 0 (i+j) -> no_loop ss size 0 i.
+Lemma split_no_loop' : forall (ss:sseq) (o i k j:nat),
+  no_loop' ss o i (j+k) -> no_loop' ss o i j.
+Proof.
+  induction k.
+  - intros.
+    rewrite -> plus_0_r in H.
+    apply H.
+  - intros.
+    rewrite <- Nat.add_succ_comm in H.
+    apply IHk in H.
+    simpl in H.
+    destruct H.
+    apply H.
+Qed.
+
+Lemma split_no_loop_former : forall (ss : sseq) (j i : nat),
+  no_loop ss 0 (i+j) -> no_loop ss 0 i.
 Proof.
   induction j.
-  - intros.  rewrite <- plus_n_O in H.
-    easy.
+  - intros.
+    now rewrite <- plus_n_O in H.
   - intros.
     rewrite <- Nat.add_succ_comm in H.
     apply IHj in H.
-    assert(no_loop ss size 0 (S i) <-> 
-      no_loop ss size 0 i /\ no_loop' ss size 0 (S i) i)
-      by (destruct i; firstorder).
-    apply H0 in H.
-    firstorder.
+    simpl in H.
+    destruct H.
+    apply H0.
 Qed.
 
+
 Local Lemma split_no_loop_latter'' : 
-  forall (ss : sseq) (size i j k : nat),
-  no_loop' ss size i (S k) (S j) <->
-    neq_states ss.[(i + (S k))] ss.[i] size /\
-    no_loop' ss size (S i) k j.
+  forall (ss : sseq) (i j k : nat),
+  no_loop' ss i (S k) (S j) <->
+    ss.[(i + (S k))] <> ss.[i] /\
+    no_loop' ss (S i) k j.
 Proof.
   destruct j.
-  - simpl. rewrite <-  plus_n_O.
+  - simpl. 
+    (*rewrite <-  plus_n_O.*)
     intros.
     now rewrite <- Nat.add_succ_l;
       rewrite Nat.add_succ_comm; rewrite Nat.add_1_r.
   - induction j.
     + simpl.
       intros.
-      do 3 rewrite <- Nat.add_succ_r.
-      rewrite <-  Nat.add_1_r; rewrite <- (plus_n_O i).
+      do 2 rewrite <- Nat.add_succ_r.
+      do 1 rewrite ->  Nat.add_1_r.
       tauto.
     + intros.
       simpl in *.
@@ -396,32 +340,32 @@ Proof.
       rewrite <- IHj.
       do 2 rewrite <- Nat.add_succ_r.
       tauto.
-Qed. (*26*)
+Qed.
 
-Local Lemma split_no_loop_latter' : forall (ss : sseq) (size j i : nat),
-  no_loop ss size i (S j) -> no_loop ss size (S i) j.
+Local Lemma split_no_loop_latter' : forall (ss : sseq) (j i : nat),
+  no_loop ss i (S j) -> no_loop ss (S i) j.
 Proof.
   induction j.
   intros.
   - destruct i; firstorder.
   - intros.
-    assert (no_loop ss size (S i) (S j) <->
-      no_loop' ss size (S i) (S j) j /\ no_loop ss size (S i) j)
+    assert (no_loop ss (S i) (S j) <->
+      no_loop' ss (S i) (S j) j /\ no_loop ss (S i) j)
       by (destruct j; firstorder).
     apply H0.
-    assert (no_loop ss size i (S (S j)) <->
-      no_loop' ss size i (S (S j)) (S j) /\ 
-      no_loop ss size i (S j))
+    assert (no_loop ss i (S (S j)) <->
+      no_loop' ss i (S (S j)) (S j) /\ 
+      no_loop ss i (S j))
       by (destruct j; firstorder).
     apply -> H1 in H.
     destruct H.
     split.
     now apply split_no_loop_latter'' in H.
     now apply IHj in H2.
-Qed. (*19*)
+Qed.
 
-Lemma split_no_loop_latter : forall (ss : sseq) (size i j : nat),
-  no_loop ss size 0 (i+j) -> no_loop ss size i j.
+Lemma split_no_loop_latter : forall (ss : sseq) (i j : nat),
+  no_loop ss 0 (i+j) -> no_loop ss i j.
 Proof.
   induction i.
   - easy.
@@ -429,30 +373,17 @@ Proof.
     rewrite Nat.add_succ_comm in H.
     apply IHi in H.
     now apply split_no_loop_latter' in H.
-Qed. (*7*)
+Qed.
 
-Lemma split_no_loop : forall (ss : sseq) (size i j: nat),
-    no_loop ss size 0 (i+j) ->
-    no_loop ss size 0 i /\ no_loop ss size i j.
+Lemma split_no_loop : forall (ss : sseq) (i j: nat),
+    no_loop ss 0 (i+j) ->
+    no_loop ss 0 i /\ no_loop ss i j.
 Proof.
   intros.
   split.
   - now apply split_no_loop_former in H.
   - now apply split_no_loop_latter in H.
 Qed.
-
-Lemma snoc_path : forall (ss : sseq) (T : trans) (i : nat),
-  path T ss 0 (S i) <->
-  path T ss 0 i /\ T ss.[i] ss.[S i].
-Proof.
-  intros. 
-  destruct i. 
-  - unfold path.
-    tauto.
-  - unfold path; fold path; simpl.
-    tauto.
-Qed. (*8*)
-
 
 Lemma cons_path : forall (ss : sseq) (T : trans) (i j : nat),
   T ss.[i] ss.[S i] /\ path T ss (S i) j <->
@@ -472,36 +403,87 @@ Proof.
     + simpl.
       split; firstorder;
       now do 5 rewrite Nat.add_succ_r in *.
-Qed. (*13*)
+Qed.
+
+(*
+Lemma snoc_path : forall (ss : sseq) (T : trans) (i : nat),
+  path T ss 0 (S i) <->
+  path T ss 0 i /\ T ss.[i] ss.[S i].
+Proof.
+  intros. 
+  destruct i. 
+  - unfold path.
+    tauto.
+  - unfold path; fold path; simpl.
+    tauto.
+Qed.
+*)
+
+Lemma snoc_path : forall (ss : sseq) (T : trans) (i j: nat),
+  path T ss i (S j) <->
+  path T ss i j /\ T ss.[i+j] ss.[S (i+j)].
+Proof.
+  intros.
+  simpl.
+  replace (i + S j) with (S (i + j)).
+  tauto.
+  auto.
+Qed.
+
+Lemma skip1_path : forall (T : trans) (i j : nat),
+  forall ss : sseq,
+  path T ss (S i) j -> path T (skipn 1 ss) i j.
+Proof.
+  intros.
+  induction j.
+  - simpl. intuition.
+  - rewrite -> snoc_path in H.
+    destruct H.
+    rewrite -> snoc_path.
+    split.
+    * apply IHj.
+      apply H.
+    * do 2 rewrite skipn_nth.
+      replace (1+(i+j)) with (S i + j).
+      replace (1+S (i+j)) with (S (S i + j)).
+      apply H0.
+      auto. 
+      auto.
+Qed.
 
 Lemma shift_path : forall (ss : sseq) (T : trans) (i j : nat), 
   path T ss 0 i /\ path T ss i (S j) <-> 
   path T ss 0 (S i) /\ path T ss (S i) j .
 Proof.
   intros.
-  rewrite snoc_path.
+  rewrite snoc_path with (i:=0).
   rewrite and_assoc.
   rewrite cons_path.
   reflexivity.
-Qed. (*5*)
+Qed.
 
 Lemma split_path : forall (ss : sseq) (T : trans) (i j: nat),
-  path T ss 0 (i+j) -> path T ss 0 i /\ path T ss i j.
+  path T ss 0 (i+j) <-> path T ss 0 i /\ path T ss i j.
 Proof.
   induction i.
   - simpl.
     tauto.
+  - split.
+    + intros.
+      rewrite -> Nat.add_succ_comm in H.
+      apply IHi in H.
+      apply shift_path.
+      apply H.
+    + intros.
+      apply shift_path in H.
+      apply IHi in H.
+      rewrite <- Nat.add_succ_comm in H.
+      apply H.
+Qed.
 
-  - intros.
-    rewrite -> Nat.add_succ_comm in H.
-    apply IHi in H.
-    apply shift_path.
-    apply H.
-Qed. (*8*)
-
-Lemma split_loop_free : forall  (ss : sseq) (T : trans) (size i j : nat),
-  loop_free T ss size 0 (i+j) -> 
-  loop_free T ss size 0 i /\ loop_free T ss size i j.
+Lemma split_loop_free : forall  (ss : sseq) (T : trans) (i j : nat),
+  loop_free T ss 0 (i+j) -> 
+  loop_free T ss 0 i /\ loop_free T ss i j.
 Proof.
   unfold loop_free.
   intros.
@@ -510,5 +492,1126 @@ Proof.
   apply split_no_loop in H0.
   tauto.
 Qed.
+
+Lemma split_path_lf :
+  forall (T:trans) (ss:sseq) (m n:nat),
+    loop_free T ss 0 m /\ path T ss m n ->
+    path T ss 0 (m+n).
+Proof.
+  induction m.
+  - intros.
+    unfold loop_free in H.
+    decompose [and] H; clear H.
+    tauto.
+  - intros.
+    unfold loop_free in H.
+    decompose [and] H; clear H.
+    assert (path T ss 0 (S m) /\ path T ss (S m) n) by auto.
+    clear H1 H2.
+    apply shift_path in H.
+    destruct H.
+    rewrite <- Nat.add_1_r in H3.
+    apply split_no_loop_former in H3.
+    assert (loop_free T ss 0 m /\ path T ss m (S n)) by (unfold loop_free; tauto).
+    clear H3 H H0.
+    apply IHm in H1.
+    rewrite <- Nat.add_succ_comm in H1.
+    apply H1.
+Qed.
+
+(*
+Lemma split_path_init_lf :
+  forall (I:init) (T:trans) (size m n:nat) (ss:sseq),
+    I ss.[0] /\ loop_free T ss size 0 m /\ path T ss m n ->
+    I ss.[0] /\ path T ss 0 (m+n).
+Proof.
+  induction m.
+  - intros.
+    (*rewrite -> Nat.add_0_r in *.*)
+    unfold loop_free in H.
+    decompose [and] H; clear H.
+    tauto.
+  - intros.
+    unfold loop_free in H.
+    decompose [and] H; clear H.
+    assert (path T ss 0 (S m) /\ path T ss (S m) n) by auto.
+    clear H3 H1.
+    apply shift_path in H.
+    (*rewrite <- Nat.add_succ_r in H.
+    rewrite -> Nat.add_succ_comm in H.*)
+    destruct H.
+    rewrite <- Nat.add_1_r in H4.
+    apply split_no_loop_former in H4.
+    assert (I ss.[0] /\ loop_free T ss size 0 m /\ path T ss m  (S n)) by (unfold loop_free; tauto).
+    clear H0 H1 H4 H.
+    apply IHm in H2.
+    rewrite <- Nat.add_succ_comm in H2.
+    apply H2.
+Qed.
+*)
+
+Lemma split_lf_path :
+  forall (T:trans) (ss:sseq) (n:nat),
+    path T ss 0 (n+1) -> 
+    ss.[n+1] <> ss.[n] ->
+    path T ss 0 n /\ loop_free T ss n 1.
+Proof.
+  induction n.
+  - intros.
+    unfold path.
+    unfold loop_free.
+    unfold no_loop.
+    unfold no_loop'.
+    rewrite -> Nat.add_0_l in *.
+    tauto.
+  - intros.
+    split.
+    + rewrite -> Nat.add_1_r in H.
+      rewrite -> snoc_path in H.
+      destruct H.
+      apply H.
+    + unfold loop_free.
+      split.
+      * rewrite -> split_path in H.
+        destruct H.
+        apply H1.
+      * unfold no_loop.
+        unfold no_loop'.
+        (*rewrite -> Nat.add_0_r.*)
+        tauto.
+Qed.
+
+(**)
+
+Lemma lf_path :
+  forall (T:trans) (ss:sseq) (i:nat),
+  loop_free T ss 0 i ->
+  path T ss 0 i.
+Proof.
+  intros.
+  induction i.
+  - simpl. intuition.
+  - simpl.
+    rewrite <- Nat.add_1_r in H.
+    apply split_loop_free in H.
+    destruct H.
+    split.
+    + apply IHi in H.
+      apply H.
+    + unfold loop_free in H0.
+      destruct H0.
+      unfold path in H0.
+      destruct H0.
+      rewrite -> Nat.add_0_r in H2.
+      rewrite -> Nat.add_1_r in H2.
+      apply H2.
+Qed.
+
+(*
+Lemma shift_path_init' :
+  forall (I:init) (T:trans) (ss:sseq) (m n:nat),
+  I ss.[m] /\ ss.[m] = ss.[n] ->
+  I ss.[n].
+Proof.
+  intros.
+  destruct H.
+  rewrite <- H0.
+  apply H.
+Qed.
+*)
+
+Lemma no_loop'_neq' :
+  forall (ss:sseq) (o i j:nat),
+  i >= j -> no_loop' ss o (S i) (i-j) ->
+  ss.[o + S i] <> ss.[o+(i-j)].
+Proof.
+  intros.
+  destruct j.
+  - destruct i.
+    + rewrite -> Nat.sub_0_r in *.
+      rewrite -> Nat.add_0_r.
+      simpl in H0.
+      apply H0.
+    + rewrite -> Nat.sub_0_r in *.
+      simpl in H0.
+      destruct H0.
+      apply H1.
+  - remember (i - S j) as k.
+    destruct k.
+    + simpl in H0.
+      rewrite -> Nat.add_0_r.
+      apply H0.
+    + simpl in H0.
+      destruct H0.
+      apply H1.
+Qed.
+
+Lemma no_loop'_neq :
+  forall (ss:sseq) (o i j:nat),
+  no_loop' ss o (S i) i ->
+  i > j -> ss.[o + S i] <> ss.[o+j].
+Proof.
+  intros.
+  remember (i-j) as k.
+  replace j with (i-k).
+  apply no_loop'_neq'.
+  omega.
+  assert (j = i - k) by omega.
+  rewrite <- H1.
+  assert (i = j + k) by omega.
+  rewrite -> H2 in H.
+  apply split_no_loop' in H.
+  rewrite <- H2 in H.
+  apply H.
+  omega.
+Qed.
+
+Lemma neq_states_no_loop' :
+  forall (ss:sseq) (o i j:nat),
+  i > j -> 
+  no_loop' ss o (S i) j -> ss.[o + S i] <> ss.[o+(S j)] ->
+  no_loop' ss o (S i) (S j).
+Proof.
+  intros.
+  destruct j.
+  - simpl.
+    split.
+    + simpl in H0.
+      apply H0.
+    + apply H1.
+  - simpl.
+    split.
+    + simpl in H0.
+      apply H0.
+    + apply H1.
+Qed.
+
+(*
+Lemma neq_states_no_loop' :
+  forall (o i:nat) (ss:sseq),
+  (forall (j:nat), i >= j -> ss.[o + S i] <> ss.[o+j]) ->
+  no_loop' ss o (S i) i.
+Proof.
+  intros.
+  unfold no_loop'.
+
+  induction i.
+  - simpl.
+    assert (ss.[o+1] <> ss.[o+0]) by (apply H; intuition).
+    rewrite -> Nat.add_0_r in H0.
+    apply H0.
+  - simpl.
+    split.
+    + unfold no_loop'.
+
+  remember (i-j) as k.
+  replace j with (i-k).
+  apply no_loop'_neq'.
+  omega.
+  assert (j = i - k) by omega.
+  rewrite <- H1.
+  assert (i = j + k) by omega.
+  rewrite -> H2 in H.
+  apply split_no_loop' in H.
+  rewrite <- H2 in H.
+  apply H.
+  omega.
+Qed.
+*)
+
+Lemma eq_states_not_no_loop' :
+  forall (ss:sseq) (o i j:nat),
+  i > j -> ss.[o + S i] = ss.[o+j] ->
+  ~ no_loop' ss o (S i) i.
+Proof.
+  intros.
+  assert (~(ss.[o + S i] <> ss.[o+j])) by tauto.
+  contradict H1.
+  apply no_loop'_neq.
+  apply H1.
+  apply H.
+Qed.
+
+Lemma lf_loop_path :
+  forall (T:trans) (i j:nat) (ss:sseq),
+  loop_free T ss 0 i -> 
+  path T ss 0 j -> ~ no_loop ss 0 j -> 
+  (* i <= j *) ~ i > j.
+Proof.
+  intros.
+  contradict H1.
+
+  unfold loop_free in H.
+  destruct H.
+
+  remember (i-j) as k.
+  assert (i = j+k) by omega.
+
+  rewrite -> H3 in H2.
+  apply split_no_loop in H2.
+  destruct H2.
+  apply H2.
+Qed.
+
+Lemma lf_loop_path' :
+  forall (T:trans) (i j:nat) (ss:sseq),
+  loop_free T ss 0 i -> 
+  i > j -> 
+  ~no_loop ss 0 j -> ~path T ss 0 j.
+Proof.
+  intros.
+  assert (~~(i > j)) by omega.
+  contradict H2.
+  revert H H2 H1.
+  apply lf_loop_path.
+Qed.
+
+Lemma lf_loop_path'' :
+  forall (T:trans) (i j:nat) (ss:sseq),
+  loop_free T ss 0 i -> 
+  path T ss 0 j -> i > j -> 
+  no_loop ss 0 j.
+Proof.
+  intros.
+  apply NNPP.
+  contradict H1.
+  revert H H0 H1.
+  apply lf_loop_path.
+Qed.
+
+(*
+Fixpoint loop' (ss : sseq) (o i j: nat) : Prop :=
+  match j with
+  | O => ss.[o+i] = ss.[o]
+  | S j' => loop' ss o i j' \/ ss.[o+i] = ss.[o+j]
+  end.
+
+Lemma not_no_loop'_loop' :
+  forall (j o i:nat) (ss:sseq),
+  ~ no_loop' ss o i j ->
+  loop' ss o i j.
+Proof.
+  induction j.
+  - intros.
+    simpl.
+    simpl in H.
+    tauto.
+  - intros.
+    simpl.
+    simpl in H.
+    apply not_and_or in H.
+    destruct H.
+    + apply IHj in H.
+      left.
+      apply H.
+    + right.
+      tauto.
+Qed.
+*)
+
+(*
+Fixpoint no_loop (ss : sseq) (o k : nat) : Prop :=
+  match k with
+  | O => True
+  | S k' => no_loop' ss o k k' /\ no_loop ss o k'
+  end.
+*)
+
+(*
+Definition eq_states (s1 s2 : state) : bool :=
+  match (s1 - s2)%Z with
+  | 0%Z => true
+  | _ => false
+  end.
+
+Fixpoint is_loop (ss : sseq) (o i j : nat) : bool :=
+  match j with
+  | O => eq_states ss.[o+i] ss.[o]
+  | S j' => if eq_states ss.[o+i] ss.[o+j] then true
+            else is_loop ss o i j'
+  end.
+
+Fixpoint find_state (ss : sseq) (o i j : nat) : nat :=
+  match j with
+  | O => i
+  | S j' => if eq_states ss.[o+i] ss.[o+j'] then j
+            else find_state ss o i j'
+  end.
+
+Fixpoint loop_state (ss : sseq) (o i : nat) : nat :=
+  match i with
+  | O => o
+  | S j => if is_loop ss o i j then i
+           else loop_state ss o j
+  end.
+*)
+
+Lemma split_skipn :
+  forall (m n i : nat) (ss : sseq),
+  (skipn (m+n) ss).[i] = (skipn m (skipn n ss)).[i].
+Proof.
+  intros.
+  do 3 rewrite -> skipn_nth.
+  assert (m + n + i = n + (m + i)) by omega.
+  rewrite -> H.
+  reflexivity.
+Qed.
+
+(*
+Require Import FunctionalExtensionality.
+
+Lemma split_skipn' :
+  forall (m n : nat) (ss : sseq),
+  (skipn (m+n) ss) = (skipn m (skipn n ss)).
+Proof.
+  intros.
+  apply functional_extensionality.
+  intros.
+  apply split_skipn.
+Qed.
+*)
+
+(*
+Definition shorter_ss' (ss1 ss2 : sseq) (o i : nat) : Prop :=
+  let i1 := loop_state ss1 o i in
+  let i2 := find_state ss1 o i1 i1 in
+  forall (j:nat), 
+    (j <= i2 /\ ss2.[j] = ss1.[j]) \/
+    (j >=  i2 /\ ss2.[j] = ss1.[i1+(j-i2)]).
+*)
+
+(*
+Definition shorter_ss (ss1 ss2 : sseq) (i d: nat) : Prop :=
+  forall (j : nat),
+  (j <= i /\ ss2.[j] = ss1.[j]) \/
+  (j >= i /\ ss2.[j] = ss1.[j+d]).
+
+Lemma skipn_shorter_ss :
+  forall (i j d : nat) (ss1 ss2 : sseq),
+  shorter_ss ss1 ss2 (i+j) d ->
+  shorter_ss (skipn i ss1) (skipn i ss2) j d.
+Proof.
+  induction i.
+  - intros.
+    rewrite -> Nat.add_0_l in H.
+    unfold shorter_ss.
+    intros.
+    do 3 rewrite -> skipn_nth.
+    do 2 rewrite -> Nat.add_0_l.
+    apply H.
+  - intros.
+    rewrite -> Nat.add_succ_comm in H.
+    apply IHi in H.
+    unfold shorter_ss.
+    intros.
+    unfold shorter_ss in H.
+    assert(S j0 <= S j /\ (skipn i ss2).[S j0] = (skipn i ss1).[S j0] \/
+       S j0 >= S j /\ (skipn i ss2).[S j0] = (skipn i ss1).[S j0 + d]) by easy.
+    destruct H0.
+    + destruct H0.
+      left.
+      split.
+      { omega. }
+      { rewrite <- Nat.add_1_l.
+        do 2 rewrite -> split_skipn.
+        do 2 rewrite -> skipn_nth with (n := 1).
+        rewrite -> Nat.add_1_l.
+        apply H1. }
+    + destruct H0.
+      { right.
+        split.
+        { omega. }
+        { rewrite <- Nat.add_1_l.
+          do 2 rewrite -> split_skipn.
+          do 2 rewrite -> skipn_nth with (n := 1).
+          rewrite -> Nat.add_1_l.
+          replace (1+(j0+d)) with (S j0 + d).
+          apply H1.
+          omega. } }
+Qed.
+
+Definition shorter_ss' (ss1 ss2 : sseq) (i d: nat) : Prop :=
+  forall (j : nat),
+  (0 < j <= i /\ ss2.[j] = ss1.[j]) \/
+  (0 < j /\ i <= j /\ ss2.[j] = ss1.[j + d]).
+
+Lemma skipn_shorter_ss' :
+  forall (i j d : nat) (ss1 ss2 : sseq),
+  shorter_ss' (skipn i ss1) (skipn i ss2) j d ->
+  shorter_ss' ss1 ss2 (i+j) d.
+Proof.
+  induction i.
+  - intros.
+    rewrite -> Nat.add_0_l.
+    unfold shorter_ss' in *.
+    intros.
+    assert (
+      0 < j0 <= j /\ (skipn 0 ss2).[j0] = (skipn 0 ss1).[j0] \/
+      0 < j0 /\ j <= j0 /\ (skipn 0 ss2).[j0] = (skipn 0 ss1).[j0 + d]) by easy.
+    do 3 rewrite -> skipn_nth in H0.
+    do 2 rewrite -> Nat.add_0_l in H0.
+    apply H0.
+  - intros.
+    rewrite -> Nat.add_succ_comm.
+
+    (* rewrite <- Nat.add_1_r in H.
+    do 2 rewrite -> split_skipn' in H.
+    apply IHi in H. 
+    *)
+
+    apply IHi.
+    unfold shorter_ss'.
+    intros.
+    unfold shorter_ss' in H.
+    assert(
+      0 < pred j0 <= j /\
+      (skipn (S i) ss2).[pred j0] = (skipn (S i) ss1).[pred j0] \/
+      0 < pred j0 /\ j <= pred j0 /\ 
+       (skipn (S i) ss2).[pred j0] = (skipn (S i) ss1).[pred j0 + d]) by easy.
+
+    destruct H0.
+    + destruct H0.
+      left; split.
+      * omega.
+      * rewrite <- Nat.add_1_l with (n := i) in H1.
+        do 2 rewrite -> split_skipn in H1.
+        do 2 rewrite -> skipn_nth with (n := 1) in H1.
+        replace (1 + pred j0) with j0 in H1.
+        apply H1.
+        omega.
+    + destruct H0.
+      right; split.
+      * omega.
+      * split.
+        { omega. }
+        { rewrite <- Nat.add_1_l with (n := i) in H1.
+          do 2 rewrite -> split_skipn in H1.
+          do 2 rewrite -> skipn_nth with (n := 1) in H1.
+          replace (1 + pred j0) with (j0) in H1.
+          replace (1 + (pred j0 + d)) with (j0+d) in H1.
+          apply H1.
+          omega. omega. }
+Qed.
+*)
+
+Definition shorter_ss_l (ss1 ss2 : sseq) (o i: nat) : Prop :=
+  forall (j : nat), j <= i-o -> ss1.[i-j] = ss2.[i-j].
+
+(*
+Definition shorter_ss_l (ss1 ss2 : sseq) (i: nat) : Prop :=
+  forall (j : nat), j <= i -> ss1.[j] = ss2.[j].
+*)
+
+Definition shorter_ss_u (ss1 ss2 : sseq) (i d: nat) : Prop :=
+  forall (j : nat), ss1.[i+j] = ss2.[i+j+d].
+
+Lemma skipn_shorter_ss_l :
+  forall (i j o : nat) (ss1 ss2 : sseq),
+  shorter_ss_l ss1 ss2 o (i+j) -> o <= i ->
+  shorter_ss_l (skipn i ss1) (skipn i ss2) 0 j.
+Proof.
+  unfold shorter_ss_l.
+  intros.
+  do 2 rewrite -> skipn_nth.
+  replace (i+(j-j0)) with (i+j-j0).
+  apply H.
+  omega.
+  omega.
+Qed.
+
+Lemma skipn_shorter_ss_l' :
+  forall (i j : nat) (ss1 ss2 : sseq),
+  shorter_ss_l (skipn i ss1) (skipn i ss2) 0 j ->
+  shorter_ss_l ss1 ss2 i (i+j).
+Proof.
+  unfold shorter_ss_l.
+  intros.
+  replace (i+j-j0) with (i+(j-j0)).
+  do 2 rewrite <- skipn_nth.
+  apply H.
+  omega.
+  omega.
+Qed.
+
+(*
+Lemma skipn_shorter_ss_l :
+  forall (i j : nat) (ss1 ss2 : sseq),
+  shorter_ss_l ss1 ss2 (i+j) ->
+  shorter_ss_l (skipn i ss1) (skipn i ss2) j.
+Proof.
+  destruct i.
+  - intros.
+    unfold shorter_ss_l in *.
+    intros.
+    do 2 rewrite -> skipn_nth.
+    do 1 rewrite -> Nat.add_0_l.
+    apply H.
+    apply H0.
+  - unfold shorter_ss_l.
+    intros.
+    assert(S i + j0 <= S i + j -> ss1.[S i + j0] = ss2.[S i + j0]) by apply H.
+    do 2 rewrite -> skipn_nth with (n := S i).
+    apply H1.
+    omega.
+Qed.
+*)
+
+Lemma skipn_shorter_ss_u :
+  forall (i j d : nat) (ss1 ss2 : sseq),
+  shorter_ss_u ss1 ss2 (i+j) d <->
+  shorter_ss_u (skipn i ss1) (skipn i ss2) j d.
+Proof.
+  unfold shorter_ss_u.
+  split.
+  - intros.
+    do 2 rewrite -> skipn_nth.
+    replace (i+(j+j0)) with (i+j+j0).
+    replace (i+(j+j0+d)) with (i+j+j0+d).
+    apply H.
+    omega.
+    omega.
+  - intros.
+    replace (i+j+j0) with (i+(j+j0)).
+    replace (i+(j+j0)+d) with (i+(j+j0+d)).
+    do 2 rewrite <- skipn_nth with (n:=i).
+    apply H.
+    omega.
+    omega.
+Qed.
+
+Lemma shorter_ss'_prop :
+  forall (P : prop) (i d : nat) (ss1 ss2 : sseq),
+  P ss1.[i] /\ shorter_ss' ss1 ss2 i d ->
+  P ss2.[i].
+Proof.
+  induction i.
+  - intros.
+    destruct H.
+    unfold shorter_ss' in H0.
+    assert (0 <= 0 /\ ss2.[0] = ss1.[0] \/
+      0 > 0 /\ ss2.[0] = ss1.[0+d]) by easy.
+    destruct H1.
+    + destruct H1.
+      rewrite -> H2.
+      apply H.
+    + destruct H1.
+      contradict H1.
+      omega.
+  - intros.
+    rewrite <- Nat.add_1_l in *.
+    rewrite <- skipn_nth in *.
+    destruct H.
+    apply skipn_shorter_ss' in H0.
+    apply IHi with (d := d) (ss1 := (skipn 1 ss1)).
+    tauto.
+Qed.
+
+Lemma shorter_ss'_prop' :
+  forall (P : prop) (i d : nat) (ss1 ss2 : sseq),
+  P ss1.[i+d+d] /\ shorter_ss' ss1 ss2 i d ->
+  P ss2.[i+d].
+Proof.
+  induction i.
+  - intros.
+    destruct H.
+    unfold shorter_ss' in H0.
+    assert (d <= 0 /\ ss2.[d] = ss1.[d] \/
+      d > 0 /\ ss2.[d] = ss1.[d+d]) by easy.
+    destruct H1.
+    + destruct H1.
+      assert (d = 0) by omega.
+      rewrite -> H3 in *.
+      do 2 rewrite -> Nat.add_0_r in *.
+      rewrite -> H2.
+      apply H.
+    + destruct H1.
+      rewrite -> Nat.add_0_l in *.
+      rewrite -> H2.
+      apply H.
+  - intros.
+    rewrite <- Nat.add_1_l in H.
+    rewrite <- skipn_nth in *.
+    destruct H.
+    apply skipn_shorter_ss' in H0.
+    rewrite <- Nat.add_1_r.
+    rewrite -> split_skipn.
+    apply skipn_shorter_ss'.
+    apply IHi with (d := d) (ss1 := (skipn 1 ss1)).
+    tauto.
+Qed.
+
+
+Lemma not_no_loop'_eq_states :
+  forall (j o i:nat) (ss:sseq),
+  ~ no_loop' ss o i j ->
+  (*
+  exists (k:nat), k <= j /\ ss.[o+i] = ss.[o+k].
+  *)
+  ~(forall (k:nat), k > j \/ ss.[o+i] <> ss.[o+k]).
+Proof.
+  induction j.
+  - intros.
+    contradict H.
+    assert (0 > 0 \/ ss.[o+i] <> ss.[o+0]) by easy.
+    destruct H0.
+    + contradict H0. omega.
+    + simpl.
+      rewrite -> Nat.add_0_r in H0.
+      apply H0.
+  - intros.
+    simpl in H.
+    apply not_and_or in H.
+    destruct H.
+    + apply IHj in H.
+      contradict H.
+      intros.
+      assert (k > S j \/ ss.[o+i] <> ss.[o+k]) by easy.
+      destruct H0.
+      * left. omega.
+      * right. apply H0.
+    + contradict H.
+      assert (S j > S j \/ ss.[o+i] <> ss.[o+S j]) by easy.
+      destruct H0.
+      * contradict H0. omega.
+      * apply H0.
+Qed.
+
+Lemma not_no_loop_eq_states :
+  forall (i o:nat) (ss:sseq),
+  ~ no_loop ss o i ->
+  (*
+  exists (ss':sseq) (k:nat), k < i /\ ss.[o+i] = ss'.[o+k].
+  *)
+  ~(forall (ss':sseq) (k:nat), k >= i \/ ss.[o+i] <> ss'.[o+k]).
+Proof.
+  induction i.
+  - intros.
+    contradict H.
+    simpl. intuition.
+  - intros.
+    simpl in H.
+    apply not_and_or in H.
+    destruct H.
+    + apply not_no_loop'_eq_states in H.
+      contradict H.
+      intros.
+      assert (k >= S i \/ ss.[o+S i] <> ss.[o+k]) by easy.
+      destruct H0.
+      * left.
+        apply H0.
+      * right.
+        apply H0.
+    + apply IHi in H.
+      contradict H.
+      intros.
+      assert (S k >= S i \/ ss.[o+S i] <> ss.[o+S k]) by easy.
+      destruct H0.
+      * left.
+        apply le_S_n in H0.
+        apply H0.
+      * Admitted.
+
+
+Lemma loop_path_prev_state :
+  forall (T:trans) (i:nat) (ss:sseq),
+  path T ss 0 i -> ~ no_loop ss 0 i ->
+  (* 
+  exists (j:nat), j < i /\ ss.[i] = ss.[j].
+  *)
+  ~(forall (j:nat), j < i -> ss.[i] <> ss.[j]).
+Proof.
+  Admitted.
+
+Lemma loop_path_prev_state' :
+  forall (T:trans) (i:nat) (ss:sseq),
+  path T ss 0 i ->
+  (forall (j:nat), j < i -> ss.[i] <> ss.[j]) ->
+  no_loop ss 0 i.
+Proof.
+  Admitted.
+
+Lemma safety_lf_not_path :
+  forall (I:init) (T:trans) (P:prop) (i j:nat),
+    prop_k_init_lf I T P i -> i > j ->
+    ~ prop_k_init I T P j.
+Proof.
+  Admitted.
+
+Lemma safety_lf_path0 :
+  forall (I:init) (T:trans) (P:prop),
+    (forall (i:nat), prop_k_init_lf I T P i) ->
+    prop_k_init I T P 0.
+Proof.
+  unfold prop_k_init.
+  unfold prop_k_init_lf.
+  intros.
+  assert ((forall (p1 p2 p3:Prop), ((p1 /\ p3 -> ~p2) <-> ~(p1 /\ p2 /\ p3)))) by tauto.
+  apply H0.
+  intros.
+  assert (~loop_free T ss 0 0).
+  { revert H1.
+    apply H0.
+    apply H. }
+  contradict H2.
+  unfold loop_free.
+  split.
+  - apply H2.
+  - simpl. intuition.
+Qed.
+
+Lemma safety_lf_path1 :
+  forall (I:init) (T:trans) (P:prop),
+    prop_k_init_lf I T P 0 ->
+    prop_k_init_lf I T P 1 ->
+    prop_k_init I T P 1.
+Proof.
+  unfold prop_k_init.
+  unfold prop_k_init_lf.
+  intros.
+  assert ((forall (p1 p2 p3:Prop), ((p1 /\ p3 -> ~p2) <-> ~(p1 /\ p2 /\ p3)))) by tauto.
+  apply H1.
+  intros.
+  assert (~loop_free T ss 0 1).
+  { revert H2.
+    apply H1.
+    apply H0. }
+  contradict H3.
+  unfold loop_free.
+  split.
+  - apply H3.
+  - simpl.
+    destruct H2.
+    split.
+    contradict H4.
+    rewrite -> H4.
+    assert (loop_free T ss 0 0) by easy.
+    revert H2 H5.
+    apply imply_not_and3.
+    apply H.
+    intuition.
+Qed.
+
+Lemma safety_lf_path :
+  forall (I:init) (T:trans) (P:prop) (k:nat),
+    (forall (j:nat), prop_k_init_lf I T P j) ->
+    (forall (j:nat), j < k -> prop_k_init I T P j) ->
+    prop_k_init I T P k.
+Proof.
+  intros.
+  unfold prop_k_init.
+  intros.
+  assert ((forall (p1 p2 p3:Prop), ((p1 /\ p3 -> ~p2) <-> ~(p1 /\ p2 /\ p3)))) by tauto.
+  apply H1.
+  intros.
+  destruct H2.
+
+  assert (~loop_free T ss 0 k).
+  { revert H2 H3.
+    assert ((forall (p1 p2 p3:Prop), (~(p1 /\ p3 /\ p2) <-> (p1 -> p2 -> ~p3)))) by tauto.
+    apply H2.
+    apply H. }
+
+  unfold loop_free in H4.
+  apply not_and_or in H4.
+  destruct H4.
+  apply H4.
+
+  contradict H4.
+
+  apply loop_path_prev_state' with (T:=T).
+  apply H4.
+  intros.
+
+  assert (prop_k_init I T P j).
+  apply H0. apply H5.
+
+  unfold prop_k_init in H6.
+
+  remember (k-j) as j'.
+  replace k with (j+j') in H4.
+  apply split_path in H4.
+  destruct H4.
+
+  assert (P ss.[j]).
+  revert H2 H4.
+  apply imply_not_and3.
+  apply H6.
+
+  contradict H3.
+  rewrite -> H3.
+  apply H8.
+
+  omega.
+Qed.
+
+Lemma safety_lf_path' :
+  forall (I:init) (T:trans) (P:prop) (k:nat),
+    (forall (j:nat), j < k -> prop_k_init I T P j) ->
+    prop_k_init_lf I T P k ->
+    prop_k_init I T P k.
+Proof.
+  intros.
+  unfold prop_k_init.
+  intros.
+  assert ((forall (p1 p2 p3:Prop), ((p1 /\ p3 -> ~p2) <-> ~(p1 /\ p2 /\ p3)))) by tauto.
+  apply H1.
+  intros.
+  destruct H2.
+
+  assert (~loop_free T ss 0 k).
+  { revert H2 H3.
+    assert ((forall (p1 p2 p3:Prop), (~(p1 /\ p3 /\ p2) <-> (p1 -> p2 -> ~p3)))) by tauto.
+    apply H2.
+    apply H0. }
+
+  unfold loop_free in H4.
+  apply not_and_or in H4.
+  destruct H4.
+  apply H4.
+
+  contradict H4.
+
+  apply loop_path_prev_state' with (T:=T).
+  apply H4.
+  intros.
+
+  assert (prop_k_init I T P j).
+  { apply H. apply H5. }
+
+  unfold prop_k_init in H6.
+
+  remember (k-j) as j'.
+  replace k with (j+j') in H4.
+  apply split_path in H4.
+  destruct H4.
+
+  assert (P ss.[j]).
+  revert H2 H4.
+  apply imply_not_and3.
+  apply H6.
+
+  contradict H3.
+  rewrite -> H3.
+  apply H8.
+
+  omega.
+Qed.
+
+
+(*
+
+Lemma safety_lf_path :
+  forall (I:init) (T:trans) (P:prop) (size:nat) (i:nat),
+    (forall (i:nat), prop_k_init_lf I T P size i) ->
+    prop_k_init I T P i.
+Proof.
+  unfold prop_k_init.
+  unfold prop_k_init_lf.
+  intros.
+  apply and_imply_not_and3.
+  intros.
+  destruct H0.
+  assert (no_loop ss size 0 i \/ ~no_loop ss size 0 i) by tauto.
+  destruct H2.
+  - assert (loop_free T ss size 0 i) by easy.
+    revert H0 H3.
+    apply imply_not_and3.
+    apply H.
+  - 
+
+
+  (*unfold prop_k_init.
+  unfold prop_k_init_lf.*)
+  induction i.
+  - unfold prop_k_init.
+    unfold prop_k_init_lf.
+    intros.
+    assert (loop_free T ss size 0 0) by easy.
+    apply and_imply_not_and3.
+    intros.
+    destruct H1.
+    revert H1 H0.
+    apply imply_not_and3.
+    apply H.
+  - intros.
+    unfold prop_k_init.
+    intros.
+    apply and_imply_not_and3.
+    intros.
+    destruct H0.
+    assert (no_loop ss size 0 (S i) \/ ~no_loop ss size 0 (S i)) by tauto.
+    destruct H2.
+    + unfold prop_k_init_lf in H.
+      assert (loop_free T ss size 0 (S i)) by easy.
+      revert H0 H3.
+      apply imply_not_and3.
+      apply H.
+
+
+    assert (neq_states ss.[S i] ss.[i] size \/
+      ~neq_states ss.[S i] ss.[i] size) by tauto.
+    destruct H2.
+    + rewrite <- Nat.add_1_r in H1.
+      (*rewrite split_path in H1.
+      destruct H1.*)
+      assert (loop_free T ss size i 1).
+      { apply split_lf_path.
+        apply H1.
+        rewrite -> Nat.add_1_r.
+        apply H2. }
+      
+      
+      assert ().
+
+
+    apply IHi.
+    apply H.
+    unfold prop_k_init.
+    intros.
+
+
+Lemma safety_lf_path' :
+  forall (I:init) (T:trans) (P:prop) (size:nat),
+    (forall (i:nat), prop_k_init_lf I T P size i) ->
+    (forall (i j:nat), i >= j -> prop_k_init I T P j).
+Proof.
+  intros.
+  unfold prop_k_init.
+  unfold prop_k_init_lf in H.
+  (*unfold loop_free in H.*)
+  intros.
+  induction i.
+  - assert (j = 0) by intuition.
+    assert (no_loop ss size 0 j) by now rewrite -> H1.
+    apply and_imply_not_and3.
+    intros.
+    destruct H3.
+    assert (loop_free T ss size 0 j) by now unfold loop_free.
+    revert H3 H5.
+    apply imply_not_and3.
+    apply H.
+  - apply IHi. Admitted.
+
+(*  - assert (loop_free T ss size 0 j \/ ~loop_free T ss size 0 j) by tauto.
+    destruct H1.
+    + apply and_imply_not_and3.
+      intros.
+      destruct H2.
+      revert H2 H1.
+      apply imply_not_and3.
+      apply H.
+    + contradict H1.
+      decompose [and] H1; clear H1.
+      unfold loop_free.
+      split.
+      * apply H4.
+      * assert (~no_loop ss size 0 j).
+        revert H2 H4 H5.
+        assert (forall (p1 p2 p3 p4:Prop), 
+          ~(p1 /\ (p2 /\ p4) /\ p3) -> (p1 -> p2 -> p3 -> ~p4)).
+        { intros. revert H2 H3 H4.
+          apply not_and_or in H1.
+          destruct H1. tauto.
+          apply not_and_or in H1.
+          destruct H1.
+          apply not_and_or in H1.
+          destruct H1. tauto.
+          tauto. tauto. }
+        apply H1.
+        apply H.
+        Admitted.
+*)
+
+(*
+Lemma safety_lf_path :
+  forall (I:init) (T:trans) (P:prop) (size:nat),
+    (forall (i:nat), prop_k_init_lf I T P size i) ->
+    (forall (i:nat), prop_k_init I T P i).
+Proof.
+  intros.
+  unfold prop_k_init.
+  unfold prop_k_init_lf in H.
+  (*unfold loop_free in H.*)
+  intros.
+  induction i.
+  - assert (no_loop ss size 0 0) by intuition.
+    apply and_imply_not_and3.
+    intros.
+    decompose [and] H1; clear H1.
+    assert (loop_free T ss size 0 0) by now unfold loop_free.
+    revert H2 H1.
+    apply imply_not_and3.
+    apply H.
+  - assert (loop_free T ss size 0 (S i) \/ ~loop_free T ss size 0 (S i)) by tauto.
+    destruct H0.
+    + apply and_imply_not_and3.
+      intros.
+      decompose [and] H1; clear H1.
+      revert H2 H0.
+      apply imply_not_and3.
+      apply H.
+    + contradict H0.
+      decompose [and] H0; clear H0.
+      unfold loop_free.
+      split.
+      * apply H3.
+      * simpl.
+
+loop_free T ss size 0 k -> 
+~(I ss.[0] /\ path T ss 0 k /\ ~P ss.[k])
+
+Lemma safety_lf_path :
+  forall (I:init) (T:trans) (P:prop) (size:nat),
+    (forall (i:nat), prop_k_init_lf I T P size i) ->
+    (forall (k i:nat), i <= k -> prop_k_init I T P i).
+Proof.
+  intros.
+  unfold prop_k_init.
+  unfold prop_k_init_lf in H.
+  (*unfold loop_free in H.*)
+  intros.
+  induction k.
+  - assert (i = 0) by intuition.
+    assert (no_loop ss size 0 i) by now rewrite -> H1.
+    apply and_imply_not_and3.
+    intros.
+    decompose [and] H3; clear H3.
+    assert (loop_free T ss size 0 i) by now unfold loop_free.
+    revert H4 H3.
+    apply imply_not_and3.
+    apply H.
+  - 
+
+
+Lemma safety_lf_path :
+  forall (I:init) (T:trans) (P:prop) (size:nat),
+    (forall (i:nat), prop_k_init_lf I T P size i) ->
+    (forall (i:nat), prop_k_init I T P i).
+Proof.
+  intros.
+  unfold prop_k_init.
+  unfold prop_k_init_lf in H.
+  (*unfold loop_free in H.*)
+  intros.
+  induction i.
+  - assert (no_loop ss size 0 0) by intuition.
+    apply and_imply_not_and3.
+    intros.
+    decompose [and] H1; clear H1.
+    assert (loop_free T ss size 0 0) by now unfold loop_free.
+    revert H2 H1.
+    apply imply_not_and3.
+    apply H.
+
+  - assert (loop_free T ss size 0 (S i) \/ ~loop_free T ss size 0 (S i)) by tauto.
+    destruct H0.
+    + apply and_imply_not_and3.
+      intros.
+      decompose [and] H1; clear H1.
+      revert H2 H0.
+      apply imply_not_and3.
+      apply H.
+    + 
+*)
 
 (* eof *)
